interface example of bisimulation

examples/ContractSystems/interface/interface.v
@@ -4,10 +4,9 @@ From ConCert.Execution Require Import ContractCommon.
 From ConCert.Execution Require Import Monad.
 From ConCert.Execution Require Import ResultMonad.
 From ConCert.Execution Require Import Serializable.
+From ConCert.Execution Require Import ChainedList.
 From ConCert.Utils Require Import RecordUpdate.
 From ConCert.Utils Require Import Extras.
-From FinCert.Meta Require Import ContractMorphisms.
-From FinCert.Meta Require Import ContractSystems.
 From Coq Require Import FunctionalExtensionality.
 From Coq Require Import Ensembles.
 From Coq Require Import ZArith_base.
@@ -18,7 +17,8 @@ From Coq Require Import Fin.
 From Coq.Init Require Import Byte.
 
 From FinCert.Meta Require Import ContractMorphisms.
-From ConCert.Execution Require Import ContractSystems.
+From FinCert.Meta Require Import ContractSystems.
+From FinCert.Meta Require Import Bisimulation.
 
 Import ListNotations.
 Open Scope N_scope.
@@ -30,7 +30,336 @@ Open Scope string.
         C_interface
              /
          C_backend
-
+    
+    Under the condition of a link graph specification, these contracts are 
 *)
 
-(* TODO *)
+Section Interface.
+Context { Base : ChainBase }.
+Set Primitive Projections.
+Set Nonrecursive Elimination Schemes.
+
+(* the various contract types *)
+Definition setup := unit.
+Inductive entrypoint := 
+| incr (n : nat).
+Record state := build_state { counter : nat }.
+Definition error := nat.
+
+(* for the interface *)
+Definition setup_i := Address.
+Inductive entrypoint_i := 
+| incr_i (n : nat).
+Record state_i := build_state_i { backend_address : Address }.
+Definition error_i := nat.
+
+(* for the backend *)
+Definition setup_b := Address.
+Inductive entrypoint_b := 
+| incr_b (n : nat).
+Record state_b := 
+    build_state_b { interface_address : Address ; counter_backend : nat }.
+Definition error_b := nat.
+
+Section Serialization.
+    Global Instance entrypoint_serializable : Serializable entrypoint := 
+        Derive Serializable entrypoint_rect<incr>.
+    Global Instance entrypoint_i_serializable : Serializable entrypoint_i := 
+        Derive Serializable entrypoint_i_rect<incr_i>.
+    Global Instance entrypoint_b_serializable : Serializable entrypoint_b := 
+        Derive Serializable entrypoint_b_rect<incr_b>.
+    Global Instance state_serializable : Serializable state := 
+        Derive Serializable state_rect<build_state>.
+    Global Instance state_i_serializable : Serializable state_i := 
+        Derive Serializable state_i_rect<build_state_i>.
+    Global Instance state_b_serializable : Serializable state_b := 
+        Derive Serializable state_b_rect<build_state_b>.
+End Serialization.
+
+
+Section Mono.
+
+(* initialize with 0 in storage *)
+Definition init 
+    (_ : Chain)
+    (_ : ContractCallContext)
+    (_ : setup) : result state error := 
+    Ok (build_state 0).
+
+(* receive *)
+Definition receive
+    (_ : Chain)
+    (_ : ContractCallContext)
+    (st : state) 
+    (msg : option entrypoint) : result (state * list ActionBody) error :=
+    match msg with 
+    | Some (incr n) => 
+        Ok (build_state (counter st + n), [])
+    | None => Err 0%nat
+    end.
+
+Definition contract_mono := build_contract init receive.
+
+End Mono.
+
+
+Section Modular.
+
+Section Interface.
+
+(* initialize with 0 in storage *)
+Definition init_i
+    (_ : Chain)
+    (_ : ContractCallContext)
+    (caddr : setup_i) : result state_i error_i := 
+    Ok (build_state_i caddr).
+
+(* receive *)
+Definition receive_i
+    (_ : Chain)
+    (_ : ContractCallContext)
+    (st : state_i) 
+    (msg : option entrypoint_i) : result (state_i * list ActionBody) error_i :=
+    match msg with
+    | Some (incr_i n) => 
+        let act_incr := act_call (backend_address st) 0 (serialize (incr_b n)) in
+        Ok (st, [ act_incr ])
+    | None => Err 0%nat
+    end.
+
+Definition contract_interface := build_contract init_i receive_i.
+
+End Interface.
+
+Section Backend.
+
+(* initialize with 0 in storage *)
+Definition init_b
+    (_ : Chain)
+    (_ : ContractCallContext)
+    (caddr : setup_b) : result state_b error_b := 
+    Ok (build_state_b caddr 0%nat).
+
+(* receive *)
+Definition receive_b
+    (_ : Chain)
+    (ctx : ContractCallContext)
+    (st : state_b) 
+    (msg : option entrypoint_b) : result (state_b * list ActionBody) error_b :=
+    if address_eqb (ctx_from ctx) (interface_address st) then 
+        match msg with 
+        | Some (incr_b n) => 
+            Ok (build_state_b (interface_address st) (counter_backend st + n), [])
+        | None => Err 0%nat
+        end
+    else Err 0%nat.
+
+Definition contract_backend := build_contract init_b receive_b.
+
+End Backend.
+
+End Modular.
+
+(* the systems in question *)
+Definition mono := singleton_sys contract_mono.
+Definition modu := nest contract_interface contract_backend.
+
+
+Section Bisimulation.
+Context {interface_caddr backend_caddr : Address}.
+
+Definition permissioned_ctx ctx := {|
+    ctx_origin := interface_caddr ;
+    ctx_from := interface_caddr ;
+    ctx_contract_address := backend_caddr ;
+    ctx_contract_balance := ctx_contract_balance ctx ; (* 0? ... *)
+    ctx_amount := 0 ;
+|}.
+
+Section LinkGraph.
+
+(* The link graph specification for mono *)
+Axiom mono_link_graph_clnil : forall st (step : SystemStep mono st st),
+    step = clnil.
+
+Axiom mono_link_graph_step : forall st1 st2 (step : SystemStep mono st1 st2),
+    exists c ctx n recv_ok,
+    let step_mono := build_sys_single_step mono st1 st2
+        c
+        ctx
+        (Some (incr n))
+        nil
+        recv_ok in 
+    step = snoc clnil step_mono.
+
+(* The link graph specification for modu *)
+Axiom modu_link_graph_clnil : forall st (step : SystemStep modu st st),
+    step = clnil.
+
+Axiom modu_link_graph_step : forall st1 st2 (step : SystemStep modu st1 st2),
+    exists c ctx n recvi_ok recvb_ok, 
+    let step_interface := build_sys_single_step modu st1 st2 
+        c
+        ctx
+        (Some (inl (incr_i n))) 
+        [act_call backend_caddr 0 (serialize (incr_b n))]
+        recvi_ok in 
+    let step_backend := build_sys_single_step modu st1 st2
+        c
+        (permissioned_ctx ctx)
+        (Some (inr (incr_b n)))
+        nil
+        recvb_ok in 
+    step = snoc (snoc clnil step_interface) step_backend.
+
+End LinkGraph.
+
+
+(* the morphisms *)
+(* mono -> modu *)
+Definition stm_mono_mod : SystemTraceMorphism mono modu.
+Proof.
+    apply (build_st_morph mono modu
+        (* the function between state types *)
+        (fun st =>
+            (build_state_i backend_caddr, build_state_b interface_caddr (counter st)))).
+    -   intros st gen_mono.
+        unfold is_genesis_sys_state in *.
+        destruct gen_mono as [c [ctx [s init_ok]]].
+        exists c, ctx, (backend_caddr, interface_caddr).
+        unfold sys_init, modu, mono in *.
+        cbn in *.
+        unfold init in init_ok.
+        now inversion init_ok.
+    -   intros st1 st2 step.
+        induction step; try apply clnil.
+        destruct l as [c ctx op_msg nacts recv_ok].
+        (* send step to *)
+        destruct op_msg.
+        2:{ (* none case *)
+            now unfold sys_receive in *. }
+        destruct e.
+        (* send the single step of the monolithic contract to a *pair* of steps
+            of the modular contract system *)
+        assert (SingleSystemStep modu 
+            ({| backend_address := backend_caddr |}, 
+                {| interface_address := interface_caddr; counter_backend := counter mid |})
+            ({| backend_address := backend_caddr |}, 
+                {| interface_address := interface_caddr; counter_backend := counter mid |}))
+        as step_interface.
+        (* first the call to the interface contract, 
+            which results in a call to the backend contract *)
+        {   apply (build_sys_single_step modu _ _ c ctx 
+                (Some (inl (incr_i n))) [act_call backend_caddr 0 (serialize (incr_b n))]).
+            now unfold sys_receive in *. }
+        apply (snoc (snoc IHstep step_interface)).
+        clear step_interface.
+        (* then the call to the backend *)
+        apply (build_sys_single_step modu _ _ c (permissioned_ctx ctx)
+            (Some (inr (incr_b n))) nil).
+        unfold sys_receive, mono, modu in *.
+        cbn in *.
+        unfold receive_b.
+        cbn.
+        rewrite (address_eq_refl interface_caddr).
+        now inversion recv_ok.
+Defined.
+
+
+(* modu -> mono *)
+Definition stm_mod_mono : SystemTraceMorphism modu mono.
+Proof.
+    apply (build_st_morph modu mono
+        (* the function between state types *)
+        (fun '(st_i, st_b) => build_state (counter_backend st_b))).
+    -   intros st gen_modu.
+        unfold is_genesis_sys_state, mono, modu in *.
+        destruct gen_modu as [c [ctx [s init_ok]]].
+        exists c, ctx, tt.
+        destruct st as [st_i st_b].
+        destruct s as [s_i s_b].
+        cbn in *.
+        unfold sys_init, nest, init in *.
+        now inversion init_ok.
+    -   intros st1 st2.
+        assert (forall P : (SystemStep modu st1 st2) -> Type,
+        forall c ctx n recvi_ok recvb_ok,
+        P (snoc (snoc clnil
+            (build_sys_single_step modu st1 st1 c ctx (Some (inl (incr_i n)))
+                [act_call backend_caddr 0 (serialize (incr_b n))]
+                recvi_ok))
+            (build_sys_single_step modu st1 st2 c (permissioned_ctx ctx)
+                (Some (inr (incr_b n))) nil
+                recvb_ok)) -> 
+        forall (step : SystemStep modu st1 st2), P step)
+        as H_modu_ind.
+        { admit. }
+        apply H_modu_ind.
+    
+        step.
+        (* by the link graph, step is either clnil or a nested pair of calls *)
+        induction step. 
+        +   admit.
+        +   
+
+        assert Chain as c. { admit. }
+        assert ContractCallContext as ctx. { admit. } 
+        assert nat as n. { admit. }
+        assert (sys_receive modu c ctx st1 (Some (inl (incr_i n))) = 
+        Ok (st1, [act_call backend_caddr 0 (serialize (incr_b n))]))
+        as recvi_ok. { admit. }
+        assert (sys_receive modu c (permissioned_ctx ctx) st1 (Some (inr (incr_b n))) = Ok (st2, []))
+        as recvb_ok. { admit. }
+        assert (step =
+        snoc
+          (snoc clnil
+             {|
+               sys_step_chain := c;
+               sys_step_ctx := ctx;
+               sys_step_msg := Some (inl (incr_i n));
+               sys_step_nacts := [act_call backend_caddr 0 (serialize (incr_b n))];
+               sys_recv_ok_step := recvi_ok
+             |})
+          {|
+            sys_step_chain := c;
+            sys_step_ctx := permissioned_ctx ctx;
+            sys_step_msg := Some (inr (incr_b n));
+            sys_step_nacts := [];
+            sys_recv_ok_step := recvb_ok
+          |})
+        as step_eq. { admit. }
+        
+        
+        assert (exists c ctx n recvi_ok recvb_ok, 
+            step = snoc (snoc clnil 
+            (build_sys_single_step modu st1 st1
+            c
+            ctx
+            (Some (inl (incr_i n))) 
+            [act_call backend_caddr 0 (serialize (incr_b n))]
+            recvi_ok)) 
+            (build_sys_single_step modu st1 st2
+            c
+            (permissioned_ctx ctx)
+            (Some (inr (incr_b n)))
+            nil
+            recvb_ok)).
+        { admit. }
+
+        apply (snoc IHstep).
+        clear IHstep.
+        destruct l as [c ctx op_msg nacts recv_ok].
+        destruct mid as [st_i_mid st_b_mid].
+        destruct to  as [st_i_to  st_b_to].
+        +   admit.
+Admitted.
+
+(* assuming the semantics of the link graph are 
+    satisfied, ...
+    
+    these systems are bisimilar. *)
+
+
+End Bisimulation.
+
+End Interface.
